specs/InteropHandler/InteropHandler/Common/block_7547743907366374244_user.lean
@@ -11,12 +11,13 @@ section
 
 open Clear EVMState Ast Expr Stmt FunctionDefinition State Interpreter ExecLemmas OutOfFuelLemmas Abstraction YulNotation PrimOps ReasoningPrinciple Utilities generated.InteropHandler InteropHandler
 
-def A_block_7547743907366374244 (s₀ s₉ : State) : Prop := sorry
-
+def A_block_7547743907366374244 (s₀ s₉ : State) : Prop :=
+  block_7547743907366374244_concrete_of_code.1 s₀ s₉
 lemma block_7547743907366374244_abs_of_concrete {s₀ s₉ : State} :
   Spec block_7547743907366374244_concrete_of_code s₀ s₉ →
   Spec A_block_7547743907366374244 s₀ s₉ := by
-  sorry
+  intro h
+  simpa [A_block_7547743907366374244] using h
 
 end
 
