specs/InteropHandler/InteropHandler/checked_sub_uint256_user.lean
@@ -11,13 +11,13 @@ section
 
 open Clear EVMState Ast Expr Stmt FunctionDefinition State Interpreter ExecLemmas OutOfFuelLemmas Abstraction YulNotation PrimOps ReasoningPrinciple Utilities InteropHandler.Common 
 
-def A_checked_sub_uint256 (diff : Identifier) (x y : Literal) (s₀ s₉ : State) : Prop := sorry
-
+def A_checked_sub_uint256 (diff : Identifier) (x y : Literal) (s₀ s₉ : State) : Prop :=
+  checked_sub_uint256_concrete_of_code.1 diff x y s₀ s₉
 lemma checked_sub_uint256_abs_of_concrete {s₀ s₉ : State} {diff x y} :
   Spec (checked_sub_uint256_concrete_of_code.1 diff x y) s₀ s₉ →
   Spec (A_checked_sub_uint256 diff x y) s₀ s₉ := by
-  unfold checked_sub_uint256_concrete_of_code A_checked_sub_uint256
-  sorry
+  intro h
+  simpa [A_checked_sub_uint256] using h
 
 end
 
