specs/InteropHandler/InteropHandler/finalize_allocation_user.lean
@@ -13,13 +13,13 @@ section
 
 open Clear EVMState Ast Expr Stmt FunctionDefinition State Interpreter ExecLemmas OutOfFuelLemmas Abstraction YulNotation PrimOps ReasoningPrinciple Utilities InteropHandler.Common 
 
-def A_finalize_allocation  (memPtr size : Literal) (s₀ s₉ : State) : Prop := sorry
-
+def A_finalize_allocation  (memPtr size : Literal) (s₀ s₉ : State) : Prop :=
+  finalize_allocation_concrete_of_code.1 memPtr size s₀ s₉
 lemma finalize_allocation_abs_of_concrete {s₀ s₉ : State} { memPtr size} :
   Spec (finalize_allocation_concrete_of_code.1  memPtr size) s₀ s₉ →
   Spec (A_finalize_allocation  memPtr size) s₀ s₉ := by
-  unfold finalize_allocation_concrete_of_code A_finalize_allocation
-  sorry
+  intro h
+  simpa [A_finalize_allocation] using h
 
 end
 
